Save the newest version

STLC/Argument.v
@@ -82,8 +82,10 @@ Fixpoint depth (func_name : string) (func_body : tm) : nat :=
        end
   | tif0 t1 t2 t3 =>
        match find_func func_name t1 with
-       | O => 1 + Coq.Arith.PeanoNat.Nat.max (depth func_name t2) (depth func_name t3)
-       | S n1 => 1 + depth func_name t1
+       | O =>
+            1 + Coq.Arith.PeanoNat.Nat.max (depth func_name t2) (depth func_name t3)
+       | S n1 =>
+            1 + Coq.Arith.PeanoNat.Nat.max (depth func_name t1) (Coq.Arith.PeanoNat.Nat.max (depth func_name t2) (depth func_name t3))
        end
   
   | tnil =>
@@ -101,19 +103,184 @@ Fixpoint depth (func_name : string) (func_body : tm) : nat :=
        end
   | tlcase t1 t2 x1 x2 t3 =>
        match find_func func_name t1 with
-       | O => 1 + Coq.Arith.PeanoNat.Nat.max (depth func_name t2) (depth func_name t3)
-       | S n1 => 1 + depth func_name t1
+       | O =>
+            1 + Coq.Arith.PeanoNat.Nat.max (depth func_name t2) (depth func_name t3)
+       | S n1 =>
+            1 + Coq.Arith.PeanoNat.Nat.max (depth func_name t1) (Coq.Arith.PeanoNat.Nat.max (depth func_name t2) (depth func_name t3))
        end
   
   | tlet _ t1 t2 =>
-       1 + Coq.Arith.PeanoNat.Nat.max (depth func_name t1) (depth func_name t2)
+       match find_func func_name t1, find_func func_name t2 with
+       | O, O =>
+            1
+       | S n1, O =>
+            1 + depth func_name t1
+       | O, S n2 =>
+            1 + depth func_name t2
+       | S n1, S n2 =>
+            1 + Coq.Arith.PeanoNat.Nat.max (depth func_name t1) (depth func_name t2)
+       end
   
   | tfix t1 =>
        1 + depth func_name t1
   end.
 
-Fixpoint CPS (k : tm) (func_name : string) (func_body : tm) (continuation : tm -> tm) (naming : nat) (fuel : nat) {struct fuel} : tm :=
+Fixpoint exact_and_subst_arg (func_name : string) (func_body : tm) (naming : nat) : tm * tm :=
+  match func_body with
+  | app t1 t2 =>
+       if is_recu func_name func_body then (func_body, var (append "res" (nat2string naming)))
+       else if is_app_F func_name func_body
+       then match find_func func_name t1 - 1 with
+            | 0 =>
+                 match find_func func_name t2 with
+                 | 0 =>
+                      (var "invalid", var "invalid")
+                 | S _ =>
+                      let (para1, para2) := exact_and_subst_arg func_name t2 naming in
+                      (para1, app t1 para2)
+                 end
+            | S _ =>
+                 let (para1, para2) := exact_and_subst_arg func_name t1 naming in
+                 (para1, app para2 t2)
+            end
+       else match find_func func_name t1 with
+            | 0 =>
+                 match find_func func_name t2 with
+                 | 0 =>
+                      (var "invalid", var "invalid")
+                 | S _ =>
+                      let (para1, para2) := exact_and_subst_arg func_name t2 naming in
+                      (para1, app t1 para2)
+                 end
+            | S _ =>
+                 let (para1, para2) := exact_and_subst_arg func_name t1 naming in
+                 (para1, app para2 t2)
+            end
+  
+  | tplus t1 t2 =>
+       match find_func func_name t1 with
+       | 0 =>
+            match find_func func_name t2 with
+            | 0 =>
+                 (var "invalid", var "invalid")
+            | S _ =>
+                 let (para1, para2) := exact_and_subst_arg func_name t2 naming in
+                 (para1, tplus t1 para2)
+            end
+       | S _ =>
+            let (para1, para2) := exact_and_subst_arg func_name t1 naming in
+            (para1, tplus para2 t2)
+       end
+  
+  | tminus t1 t2 =>
+       match find_func func_name t1 with
+       | 0 =>
+            match find_func func_name t2 with
+            | 0 =>
+                 (var "invalid", var "invalid")
+            | S _ =>
+                 let (para1, para2) := exact_and_subst_arg func_name t2 naming in
+                 (para1, tminus t1 para2)
+            end
+       | S _ =>
+            let (para1, para2) := exact_and_subst_arg func_name t1 naming in
+            (para1, tminus para2 t2)
+       end
+  
+  | tmult t1 t2 =>
+       match find_func func_name t1 with
+       | 0 =>
+            match find_func func_name t2 with
+            | 0 =>
+                 (var "invalid", var "invalid")
+            | S _ =>
+                 let (para1, para2) := exact_and_subst_arg func_name t2 naming in
+                 (para1, tmult t1 para2)
+            end
+       | S _ =>
+            let (para1, para2) := exact_and_subst_arg func_name t1 naming in
+            (para1, tmult para2 t2)
+       end
+  
+  | tif0 t1 t2 t3 =>
+       match find_func func_name t1 with
+       | 0 =>
+            match find_func func_name t2 with
+            | 0 =>
+                 match find_func func_name t3 with
+                 | 0 =>
+                      (var "invalid", var "invalid")
+                 | S _ =>
+                      let (para1, para2) := exact_and_subst_arg func_name t3 naming in
+                      (para1, tif0 t1 t2 para2)
+                 end
+            | S _ =>
+                 let (para1, para2) := exact_and_subst_arg func_name t2 naming in
+                 (para1, tif0 t1 para2 t3)
+            end
+       | S _ =>
+            let (para1, para2) := exact_and_subst_arg func_name t1 naming in
+            (para1, tif0 para2 t2 t3)
+       end
+  
+  | tcons t1 t2 =>
+       match find_func func_name t1 with
+       | 0 =>
+            match find_func func_name t2 with
+            | 0 => (var "invalid", var "invalid")
+            | S _ =>
+                 let (para1, para2) := exact_and_subst_arg func_name t2 naming in
+                 (para1, tcons t1 para2)
+            end
+       | S _ =>
+            let (para1, para2) := exact_and_subst_arg func_name t1 naming in
+            (para1, tcons para2 t2)
+       end
+  
+  | tlcase t1 t2 x1 x2 t3 =>
+       match find_func func_name t1 with
+       | 0 =>
+            match find_func func_name t2 with
+            | 0 =>
+                 match find_func func_name t3 with
+                 | 0 =>
+                      (var "invalid", var "invalid")
+                 | S _ =>
+                      let (para1, para2) := exact_and_subst_arg func_name t3 naming in
+                      (para1, tlcase t1 t2 x1 x2 para2)
+                 end
+            | S _ =>
+                 let (para1, para2) := exact_and_subst_arg func_name t2 naming in
+                 (para1, tlcase t1 para2 x1 x2 t3)
+            end
+       | S _ =>
+            let (para1, para2) := exact_and_subst_arg func_name t1 naming in
+            (para1, tlcase para2 t2 x1 x2 t3)
+       end
+  | _ =>
+       (var "invalid", var "invalid")
+  end.
+
+Fixpoint CPS_app_F (k : tm) (func_name : string) (func_body : tm) (continuation1 continuation2 : tm -> tm) (naming : nat) (fuel : nat) : tm :=
 match fuel with | 0 => func_body | S fuel' =>
+  let continuation_name := (append "res" (nat2string naming)) in
+  match find_func func_name func_body - 1 with
+  | 0 =>
+       let result := continuation1 continuation_name in
+       match find_func func_name result with
+       | 0 =>
+            continuation2 (app func_body (abs continuation_name (app k result)))
+       | S _ =>
+            continuation2 (app func_body (abs continuation_name result))
+       end
+  | S _ =>
+       let (arg, new_body) := exact_and_subst_arg func_name func_body naming in
+       let new_continuation := fun res => continuation2 (app arg (abs continuation_name res)) in
+       CPS_app_F k func_name new_body continuation1 new_continuation (naming + 1) fuel'
+  end
+end.
+
+Fixpoint CPS (k : tm) (func_name : string) (func_body : tm) (continuation : tm -> tm) (naming : nat) : tm :=
   match func_body with
   | var _ =>
        let result := continuation func_body in
@@ -122,40 +289,21 @@ match fuel with | 0 => func_body | S fuel' =>
        | S n1 => result
        end
   | abs x1 t1 =>
-       abs x1 (CPS k func_name t1 continuation naming fuel')
+       abs x1 (CPS k func_name t1 continuation naming)
   | app t1 t2 =>
-       if is_recu func_name func_body then
-       let para_name := append "res" (nat2string naming) in
-       let result := continuation (var para_name) in
-       app func_body (abs para_name
-                      match find_func func_name result with
-                      | O => app k result
-                      | S n1 => result
-                      end)
-       else if is_app_F func_name func_body
-       then match (find_func func_name t1 - 1), find_func func_name t2 with
-       | O, O =>
-            app k (continuation func_body) (*impossible*)
-       | S n1, O =>
-            CPS k func_name t1 (fun res : tm => continuation (app res t2)) naming fuel'
-       | O, S n2 =>
-            CPS k func_name t2 (fun res : tm => continuation (app t1 res)) naming fuel'
-       | S n1, S n2 =>
-            CPS k func_name t1
-            (fun res1 : tm => CPS k func_name t2
-            (fun res2 : tm => continuation (app res1 res2)) (naming + (S n1)) fuel') naming fuel'
-       end
+       if is_app_F func_name func_body
+       then CPS_app_F k func_name func_body continuation (fun res : tm => res) naming 999
        else match find_func func_name t1, find_func func_name t2 with
        | O, O =>
             app k (continuation func_body)
        | S n1, O =>
-            CPS k func_name t1 (fun res : tm => continuation (app res t2)) naming fuel'
+            CPS k func_name t1 (fun res : tm => continuation (app res t2)) naming
        | O, S n2 =>
-            CPS k func_name t2 (fun res : tm => continuation (app t1 res)) naming fuel'
+            CPS k func_name t2 (fun res : tm => continuation (app t1 res)) naming
        | S n1, S n2 =>
             CPS k func_name t1
             (fun res1 : tm => CPS k func_name t2
-            (fun res2 : tm => continuation (app res1 t2)) (naming + (S n1)) fuel') naming fuel'
+            (fun res2 : tm => continuation (app res1 res2)) (naming + (S n1))) naming
        end
   
   | tconst n =>
@@ -169,44 +317,48 @@ match fuel with | 0 => func_body | S fuel' =>
        | O, O =>
             app k (continuation func_body)
        | S n1, O =>
-            CPS k func_name t1 (fun res : tm => continuation (tplus res t2)) naming fuel'
+            CPS k func_name t1 (fun res : tm => continuation (tplus res t2)) naming
        | O, S n2 =>
-            CPS k func_name t2 (fun res : tm => continuation (tplus t1 res)) naming fuel'
+            CPS k func_name t2 (fun res : tm => continuation (tplus t1 res)) naming
        | S n1, S n2 =>
             CPS k func_name t1
             (fun res1 : tm => CPS k func_name t2
-            (fun res2 : tm => continuation (tplus res1 res2)) (naming + (S n1)) fuel') naming fuel'
+            (fun res2 : tm => continuation (tplus res1 res2)) (naming + (S n1))) naming
        end
   | tminus t1 t2 =>
        match find_func func_name t1, find_func func_name t2 with
        | O, O =>
             app k (continuation func_body)
        | S n1, O =>
-            CPS k func_name t1 (fun res : tm => continuation (tminus res t2)) naming fuel'
+            CPS k func_name t1 (fun res : tm => continuation (tminus res t2)) naming
        | O, S n2 =>
-            CPS k func_name t2 (fun res : tm => continuation (tminus t1 res)) naming fuel'
+            CPS k func_name t2 (fun res : tm => continuation (tminus t1 res)) naming
        | S n1, S n2 =>
             CPS k func_name t1
             (fun res1 : tm => CPS k func_name t2
-            (fun res2 : tm => continuation (tminus res1 res2)) (naming + (S n1)) fuel') naming fuel'
+            (fun res2 : tm => continuation (tminus res1 res2)) (naming + (S n1))) naming
        end
   | tmult t1 t2 =>
        match find_func func_name t1, find_func func_name t2 with
        | O, O =>
             app k (continuation func_body)
        | S n1, O =>
-            CPS k func_name t1 (fun res : tm => continuation (tmult res t2)) naming fuel'
+            CPS k func_name t1 (fun res : tm => continuation (tmult res t2)) naming
        | O, S n2 =>
-            CPS k func_name t2 (fun res : tm => continuation (tmult t1 res)) naming fuel'
+            CPS k func_name t2 (fun res : tm => continuation (tmult t1 res)) naming
        | S n1, S n2 =>
             CPS k func_name t1
             (fun res1 : tm => CPS k func_name t2
-            (fun res2 : tm => continuation (tmult res1 res2)) (naming + (S n1)) fuel') naming fuel'
+            (fun res2 : tm => continuation (tmult res1 res2)) (naming + (S n1))) naming
        end
   | tif0 t1 t2 t3 =>
        match find_func func_name t1 with
-       | O => tif0 t1 (CPS k func_name t2 continuation naming fuel') (CPS k func_name t3 continuation naming fuel')
-       | S n1 => CPS k func_name t1 (fun res : tm => continuation (tif0 res t2 t3)) naming fuel'
+       | O =>
+            tif0 t1 (CPS k func_name t2 continuation naming) (CPS k func_name t3 continuation naming)
+       | S n1 =>
+            CPS (abs res res) func_name t1 (fun res : tm => tif0 res
+            (CPS k func_name t2 continuation (naming + (S n1)))
+            (CPS k func_name t3 continuation (naming + (S n1)))) naming
        end
   
   | tnil =>
@@ -220,51 +372,136 @@ match fuel with | 0 => func_body | S fuel' =>
        | O, O =>
             app k (continuation func_body)
        | S n1, O =>
-            CPS k func_name t1 (fun res : tm => continuation (tcons res t2)) naming fuel'
+            CPS k func_name t1 (fun res : tm => continuation (tcons res t2)) naming
        | O, S n2 =>
-            CPS k func_name t2 (fun res : tm => continuation (tcons t1 res)) naming fuel'
+            CPS k func_name t2 (fun res : tm => continuation (tcons t1 res)) naming
        | S n1, S n2 =>
             CPS k func_name t1
             (fun res1 : tm => CPS k func_name t2
-            (fun res2 : tm => continuation (tcons res1 res2)) (naming + (S n1)) fuel') naming fuel'
+            (fun res2 : tm => continuation (tcons res1 res2)) (naming + (S n1))) naming
        end
   | tlcase t1 t2 x1 x2 t3 =>
        match find_func func_name t1 with
-       | O => tlcase t1 (CPS k func_name t2 continuation naming fuel') x1 x2 (CPS k func_name t3 continuation naming fuel')
-       | S n1 => CPS k func_name t1 (fun res : tm => continuation (tlcase res t2 x1 x2 t3)) naming fuel'
+       | O =>
+            tlcase t1 (CPS k func_name t2 continuation naming) x1 x2 (CPS k func_name t3 continuation naming)
+       | S n1 =>
+            CPS (abs res res) func_name t1 (fun res : tm => tlcase res
+            (CPS k func_name t2 continuation (naming + (S n1))) x1 x2
+            (CPS k func_name t3 continuation (naming + (S n1)))) naming
        end
   
   | tlet x1 t1 t2 =>
-       tlet x1 (CPS k func_name t1 continuation naming fuel') (CPS k func_name t2 continuation naming fuel')
+       match find_func func_name t1, find_func func_name t2 with
+       | O, O =>
+            app k (continuation func_body)
+       | S n1, O =>
+            CPS (abs res res) func_name t1 (fun res : tm => continuation (tlet x1 res (app k t2))) naming
+       | O, S n2 =>
+            CPS k func_name t2 (fun res : tm => continuation (tlet x1 t1 res)) naming
+       | S n1, S n2 =>
+              CPS (abs res res) func_name t1
+              (fun res1 : tm => CPS k func_name t2
+              (fun res2 : tm => continuation (tlet x1 res1 res2)) (naming + (S n1))) naming
+       end
   
   | tfix t1 =>
-       tfix (CPS k func_name t1 continuation naming fuel')
-  end
-end.
+       tfix (CPS k func_name t1 continuation naming)
+  end.
 
 Definition CPS_conversion (func : tm) : tm :=
   match func with
   | tfix (abs func_name func_body) =>
        let func_paraed_body := para_insert k func_body in
-       tfix (abs func_name (CPS k func_name func_paraed_body (fun res : tm => res) 1 (depth func_name func_paraed_body)))
+       tfix (abs func_name (CPS k func_name func_paraed_body (fun res : tm => res) 1))
   | _ => func
   end.
 
-Definition stlc_argument_case4 :=
-  tfix (abs F
-    (abs a
-      (abs b
-        (abs c
-          (tif0 b 3
-            (tplus 1 <{ F (F a (b - 1) c - 2) (F (a - 1) (b - 1) c - 1) (F (a - 1) (b - 2) (c - 1) - 3) }>)))))).
-
-Compute (CPS_conversion stlc_argument_case4). 
-
-Compute (CPS (var k) "F"
-<{ F (F a (b - 1) c - 2) (F (a - 1) (b - 1) c - 1) }>
-(fun res : tm => tplus 1 res) 1 999).
-
 Module examples.
+
+Definition stlc_match_case1 :=
+  tfix (abs F
+    (abs l
+      (tlcase l 0 n1 l1
+        (tlcase l1 n1 n2 l2
+          (tplus n1 (tplus n2 (app F l2))))))).
+
+Compute (CPS_conversion stlc_match_case1).
+
+Theorem stlc_match_case1_correct :
+  let origin_fun := stlc_match_case1 in
+  let CPS_fun := CPS_conversion stlc_match_case1 in
+  let input := tcons 4 (tcons 3 (tcons 1 (tcons 2 tnil))) in
+  let output := 10 in
+  (<{origin_fun input}> -->* output) /\ (<{CPS_fun input idNat}> -->* output).
+Proof. split. solve_CPS. solve_CPS. Qed.
+
+Definition stlc_match_case2 :=
+  tfix (abs F
+    (abs l
+      (tplus 1 (tlcase l 0 n1 l1
+        (tplus n1 (app F l1)))))).
+
+Compute (CPS_conversion stlc_match_case2).
+
+Theorem stlc_match_case2_correct :
+  let origin_fun := stlc_match_case2 in
+  let CPS_fun := CPS_conversion stlc_match_case2 in
+  let input := tcons 4 (tcons 3 (tcons 1 (tcons 2 tnil))) in
+  let output := 15 in
+  (<{origin_fun input}> -->* output) /\ (<{CPS_fun input idNat}> -->* output).
+Proof. split. solve_CPS. solve_CPS. Qed.
+
+Definition stlc_match_case3 :=
+  tfix (abs F
+    (abs l
+      (tlcase l 0 n1 l1
+        (tif0 (app F l1) n1 (tmult 2 n1))))).
+
+Compute (CPS_conversion stlc_match_case3).
+
+Theorem stlc_match_case3_correct :
+  let origin_fun := stlc_match_case3 in
+  let CPS_fun := CPS_conversion stlc_match_case3 in
+  let input := tcons 2 (tcons 2 tnil) in
+  let output := 4 in
+  (<{origin_fun input}> -->* output) /\ (<{CPS_fun input idNat}> -->* output).
+Proof. split. solve_CPS. solve_CPS. Qed.
+
+Definition stlc_match_case4 :=
+  tfix (abs F
+    (abs l1
+       (abs l2
+         (tplus (tlcase l1 0 n1 l'
+           (tplus n1 (app (app F l') l2)))
+             (tlcase l2 0 n2 l''
+               (tplus n2 (app (app F l1) l''))))))).
+
+Compute (CPS_conversion stlc_match_case4).
+
+Theorem stlc_match_case4_correct :
+  let origin_fun := stlc_match_case4 in
+  let CPS_fun := CPS_conversion stlc_match_case4 in
+  let input1 := tcons 2 (tcons 3 (tcons 5 tnil)) in
+  let input2 := tcons 4 (tcons 2 tnil) in
+  let output := 110 in
+  (<{origin_fun input1 input2}> -->* output) /\ (<{CPS_fun input1 input2 idNat}> -->* output).
+Proof. split. solve_CPS. solve_CPS. Qed.
+
+Definition stlc_match_case5 :=
+  tfix (abs F
+    (abs l
+      (tplus 3 (tmult (tlcase l (tminus 2 1) n1 l'
+        (tplus n1 (tplus 1 (tplus (app F l') 1)))) 5)))).
+
+Compute (CPS_conversion stlc_match_case5).
+
+Theorem stlc_match_case5_correct :
+  let origin_fun := stlc_match_case5 in
+  let CPS_fun := CPS_conversion stlc_match_case5 in
+  let input := tcons 2 (tcons 3 (tcons 5 tnil)) in
+  let output := 2113 in
+  (<{origin_fun input}> -->* output) /\ (<{CPS_fun input idNat}> -->* output).
+Proof. split. solve_CPS. solve_CPS. Qed.
 
 (*
   F n1 n2 :=
@@ -402,13 +639,13 @@ Proof. split. solve_CPS. solve_CPS. Qed.
 (*
   F a b c :=
     match b with
-    | 0 => 3
+    | 0 => 1
     | S _ => 1 + f (f a (b - 1) c - 2) (f (a - 1) (b - 1) c - 1) (f (a - 1) (b - 2) (c - 1) - 3)
     end.
   We can transfer it to CPS-style by hand:
   F a b c k :=
     match b with
-    | 0 => k 3
+    | 0 => k 1
     | S _ => f a (b - 1) c (fun res1 => f (a - 1) (b - 1) c (fun res2 => f (a - 1) (b - 2) (c - 1)
              (fun res3 => f (res1 - 2) (res2 - 1) (res3 - 3) (fun res4 => k (1 + res4)))))
     end.
@@ -419,19 +656,20 @@ Definition stlc_argument_case4 :=
     (abs a
       (abs b
         (abs c
-          (tif0 b 3
+          (tif0 b 1
             (tplus 1 <{ F (F a (b - 1) c - 2) (F (a - 1) (b - 1) c - 1) (F (a - 1) (b - 2) (c - 1) - 3) }>)))))).
 
 Compute (CPS_conversion stlc_argument_case4).
 
-Theorem stlc_argument_case3_correct :
-  let origin_fun := stlc_argument_case3 in
-  let CPS_fun := CPS_conversion stlc_argument_case3 in
-  let input := tcons 2 (tcons 3 (tcons 5 tnil)) in
-  let output := 54 in
-  (<{origin_fun input}> -->* output) /\ (<{CPS_fun input idNat}> -->* output).
+Theorem stlc_argument_case4_correct :
+  let origin_fun := stlc_argument_case4 in
+  let CPS_fun := CPS_conversion stlc_argument_case4 in
+  let input1 := 1 in
+  let input2 := 1 in
+  let input3 := 1 in
+  let output := 2 in
+  (<{origin_fun input1 input2 input3}> -->* output) /\ (<{CPS_fun input1 input2 input3 idNat}> -->* output).
 Proof. split. solve_CPS. solve_CPS. Qed.
 
-
-
 End examples.
+*)
