STLC/Proof.v
@@ -58,7 +58,7 @@ Inductive stlc_expr (func_name : string) : tm -> Prop :=
        stlc_expr func_name t2 ->
        stlc_expr func_name t3 ->
        stlc_expr func_name (tlcase t1 t2 x1 x2 t3)
-
+  
   | E_Let : forall x1 t1 t2,
        eqb func_name x1 = false ->
        stlc_expr func_name t1 ->
@@ -142,6 +142,58 @@ Inductive stlc_eqb : tm -> tm -> Prop :=
 
   where "t1 '=s' t2" := (stlc_eqb t1 t2).
 
+Inductive no_duplicate (s : string) : tm -> Prop :=
+  | D_Var : forall x1,
+       no_duplicate s (var x1)
+  | D_Abs : forall x1 t1,
+       s <> x1 ->
+       no_duplicate s t1 ->
+       no_duplicate s (abs x1 t1)
+  | D_App : forall t1 t2,
+       no_duplicate s t1 ->
+       no_duplicate s t2 ->
+       no_duplicate s (app t1 t2)
+  | D_Const : forall n,
+       no_duplicate s (tconst n)
+  | D_Plus : forall t1 t2,
+       no_duplicate s t1 ->
+       no_duplicate s t2 ->
+       no_duplicate s (tplus t1 t2)
+  | D_Minus : forall t1 t2,
+       no_duplicate s t1 ->
+       no_duplicate s t2 ->
+       no_duplicate s (tminus t1 t2)
+  | D_Mult : forall t1 t2,
+       no_duplicate s t1 ->
+       no_duplicate s t2 ->
+       no_duplicate s (tmult t1 t2)
+  | D_If0 : forall t1 t2 t3,
+       no_duplicate s t1 ->
+       no_duplicate s t2 ->
+       no_duplicate s t3 ->
+       no_duplicate s (tif0 t1 t2 t3)
+  | D_Nil :
+       no_duplicate s tnil
+  | D_Cons : forall t1 t2,
+       no_duplicate s t1 ->
+       no_duplicate s t2 ->
+       no_duplicate s (tcons t1 t2)
+  | D_LCase : forall t1 t2 x1 x2 t3,
+       s <> x1 ->
+       s <> x2 ->
+       no_duplicate s t1 ->
+       no_duplicate s t2 ->
+       no_duplicate s t3 ->
+       no_duplicate s (tlcase t1 t2 x1 x2 t3)
+  | D_Let : forall x1 t1 t2,
+       s <> x1 ->
+       no_duplicate s t1 ->
+       no_duplicate s t2 ->
+       no_duplicate s (tlet x1 t1 t2)
+  | D_Fix : forall t1,
+       no_duplicate s t1 ->
+       no_duplicate s (tfix t1).
+
 Lemma depth_helper1 :
   forall m, exists n, S m = S n.
 Proof.
@@ -157,7 +209,7 @@ Proof.
 Qed.
 
 Lemma depth_helper2 :
-  forall n m, exists k, n + k = Init.Nat.max n m.
+  forall n m, exists k, n + k = Nat.max n m.
 Proof.
   Search "<=". intros. induction (Nat.le_max_l n m).
   - exists 0. apply Nat.add_comm.
@@ -173,9 +225,22 @@ Theorem fuel_enough :
 Proof.
   intros. generalize dependent naming. generalize dependent continuation. generalize dependent n. induction M.
   - intros n H naming. destruct (depth_gt_1 F <{ s }>). rewrite H0. simpl. apply S_Refl.
-  - admit.
-  - intros n H naming. destruct (depth_gt_1 F <{ \ s, M }>). simpl in H0. injection H0 as H0. simpl. apply S_Abs. apply IHM.
-  - intros. simpl. apply S_Refl.
+  - assert (Heq : forall n m, (S n =? S m) = (n =? m)). { intros n1 m1. simpl. reflexivity. }
+    intros n H naming. destruct (depth_gt_1 F <{ M1 M2 }>). rewrite H0. simpl in H0. destruct ((find_func F M1 =? 1) && (find_func F M2 =? 0) && is_recu F M1)%bool eqn:HE.
+    injection H0 as H0. rewrite <- H0. simpl. rewrite HE. apply S_Refl. simpl. destruct (find_func F M1), (find_func F M2); simpl. apply S_Refl. injection H0 as H0. destruct (is_app_F F M1). rewrite <- H0.
+    apply IHM2. rewrite <- H0. apply IHM2. apply Bool.andb_false_iff in HE. destruct HE. apply Bool.andb_false_iff in H1. destruct H1.
+    rewrite Heq in H1. rewrite H1. simpl. destruct (is_app_F F M1). destruct n0. discriminate H1. simpl. injection H0 as H0. rewrite <- H0. apply IHM1. injection H0 as H0. rewrite <- H0. apply IHM1. discriminate H1. rewrite H1.
+    rewrite Bool.andb_comm. simpl. destruct (is_app_F F M1). destruct n0. simpl. apply S_Refl. simpl. injection H0 as H0. rewrite <- H0. apply IHM1. injection H0 as H0. rewrite <- H0. apply IHM1. rewrite (Bool.andb_comm (n0 =? 0)). simpl.
+    destruct (is_app_F F M1). destruct n0. simpl. injection H0 as H0. apply eq_sym in H0. destruct (depth_helper2 (depth F M2) (S (depth F M1))). rewrite H0. rewrite <- H1. eapply S_Trans. apply S_Symm. apply IHM2.
+    rewrite Plus.plus_assoc_reverse. apply IHM2. simpl. assert ((fun res1 : tm => CPS k F M2 (fun res2 : tm => H <{ res1 res2 }>) (naming + S n0) x) = (fun res1 : tm => CPS k F M2 (fun res2 : tm => H <{ res1 res2 }>) (naming + S n0) (x + n))). {
+    apply stlc_functional_extensionality. intros. injection H0 as H0. rewrite <- H0. destruct (depth_helper2 (depth F M2) (S (depth F M1))). rewrite <- H1. eapply S_Trans. apply S_Symm. apply IHM2. rewrite Plus.plus_assoc_reverse. apply IHM2. }
+    rewrite H1. injection H0 as H0. rewrite <- H0. destruct (depth_helper2 (S (depth F M1)) (depth F M2)). rewrite Nat.max_comm in H2. rewrite <- H2. eapply S_Trans. apply S_Symm. Search (S _ + _). rewrite Nat.add_succ_comm. apply IHM1. assert (S (depth F M1) + x0 + n = depth F M1 + S (x0 + n)). {
+    rewrite Plus.plus_assoc_reverse. apply Nat.add_succ_comm. } rewrite H3. assert (depth F M1 + S x0 + n = depth F M1 + S (x0 + n)). { rewrite Plus.plus_assoc_reverse. simpl. reflexivity. } rewrite H4. apply IHM1.
+    assert ((fun res1 : tm => CPS k F M2 (fun _ : tm => H <{ res1 M2 }>) (naming + S n0) x) = (fun res1 : tm => CPS k F M2 (fun _ : tm => H <{ res1 M2 }>) (naming + S n0) (x + n))). { apply stlc_functional_extensionality. intros. injection H0 as H0. rewrite <- H0. destruct (depth_helper2 (depth F M2) (S (depth F M1))).
+    rewrite <- H1. eapply S_Trans. apply S_Symm. apply IHM2. rewrite Plus.plus_assoc_reverse. apply IHM2. } rewrite H1. injection H0 as H0. rewrite <- H0. destruct (depth_helper2 (S (depth F M1)) (depth F M2)). rewrite Nat.max_comm in H2. rewrite <- H2. eapply S_Trans. Search (S _ + _). rewrite Nat.add_succ_comm. apply S_Symm. apply IHM1.
+    rewrite Plus.plus_assoc_reverse. rewrite (Nat.add_succ_comm (depth F M1)). rewrite Plus.plus_assoc_reverse. apply IHM1.
+  - intros. simpl. apply S_Abs. apply IHM.
+  - intros. simpl. destruct (find_func F (continuation n)). apply S_Refl. apply S_Refl.
   - intros n H naming. destruct (depth_gt_1 F <{ M1 + M2 }>). rewrite H0. simpl in H0. simpl. destruct (find_func F M1), (find_func F M2); injection H0 as H0; try (rewrite <- H0).
     apply S_Refl. apply IHM2. apply IHM1. destruct (depth_helper2 (depth F M1) (depth F M2)). rewrite <- H1. eapply S_Trans. apply S_Symm. apply IHM1. rewrite Plus.plus_assoc_reverse.
     assert ((fun res1 : tm => CPS k F M2 (fun res2 : tm => H <{ res1 + res2 }>) (naming + S n0) (depth F M1 + x0)) = (fun res1 : tm => CPS k F M2 (fun res2 : tm => H <{ res1 + res2 }>) (naming + S n0) (depth F M1 + (x0 + n)))). {
@@ -206,39 +271,140 @@ Proof.
   - intros n H naming. simpl. apply S_Let. destruct (depth_helper2 (depth F M1) (depth F M2)). rewrite <- H0. eapply S_Trans. apply S_Symm. apply IHM1. rewrite Plus.plus_assoc_reverse. apply IHM1.
     destruct (depth_helper2 (depth F M2) (depth F M1)). rewrite Nat.max_comm in H0. rewrite <- H0. eapply S_Trans. apply S_Symm. apply IHM2. rewrite Plus.plus_assoc_reverse. apply IHM2.
   - intros n H naming. simpl. apply S_Fix. apply IHM.
-  Admitted.
+Qed.
 
 Theorem naming_arbitrarility :
-  forall k F M continuation n,
-  CPS k F M continuation 1 (depth F M) =s CPS k F M continuation (1 + n) (depth F M).
-
-Theorem CPS_conversion_correct : forall F f f' k M,
-  subst F f k =s k ->
-  subst F f' k =s k ->
-  stlc_expr F M ->
-  subst F f' (CPS k F M (fun res => res) 1 (depth F M)) =s app k (subst F f M).
+  forall k F M continuation fuel n,
+  CPS k F M continuation 1 fuel =s CPS k F M continuation (1 + n) fuel.
 Proof.
-  intros. rename H into Hkf. rename H0 into Hkf'. rename H1 into H. remember M as HM. induction M; rewrite HeqHM in *; simpl.
-  - inversion H. rewrite (eqb_sym s F). rewrite H1. simpl. rewrite H1. apply S_App. apply Hkf'. apply S_Refl.
-  - admit.
-  - inversion H.
-  - apply S_App. apply Hkf'. apply S_Refl.
-  - Admitted.
+  intros. generalize dependent n. generalize dependent continuation. generalize dependent fuel. induction M; intros.
+  - destruct fuel. simpl. apply S_Refl. simpl. destruct (find_func F (continuation s)). apply S_Refl. apply S_Refl.
+  - destruct fuel. simpl. apply S_Refl. simpl. admit.
+  - destruct fuel. simpl. apply S_Refl. simpl. apply S_Abs. apply IHM.
+  - destruct fuel. simpl. apply S_Refl. simpl. destruct (find_func F (continuation n)). apply S_Refl. apply S_Refl.
+  - destruct fuel. simpl. apply S_Refl. simpl. destruct (find_func F M1), (find_func F M2). apply S_Refl. apply IHM2. apply IHM1.
+    assert (HF : (fun res1 : tm => CPS k F M2 (fun res2 : tm => continuation <{ res1 + res2 }>) (S (S n0)) fuel) = (fun res1 : tm => CPS k F M2 (fun res2 : tm => continuation <{ res1 + res2 }>) (S (n + S n0)) fuel)). {
+    apply stlc_functional_extensionality. intros. eapply S_Trans. apply S_Symm. apply IHM2. apply IHM2. } rewrite HF. apply IHM1.
+  - destruct fuel. simpl. apply S_Refl. simpl. destruct (find_func F M1), (find_func F M2). apply S_Refl. apply IHM2. apply IHM1.
+    assert (HF : (fun res1 : tm => CPS k F M2 (fun res2 : tm => continuation <{ res1 - res2 }>) (S (S n0)) fuel) = (fun res1 : tm => CPS k F M2 (fun res2 : tm => continuation <{ res1 - res2 }>) (S (n + S n0)) fuel)). {
+    apply stlc_functional_extensionality. intros. eapply S_Trans. apply S_Symm. apply IHM2. apply IHM2. } rewrite HF. apply IHM1.
+  - destruct fuel. simpl. apply S_Refl. simpl. destruct (find_func F M1), (find_func F M2). apply S_Refl. apply IHM2. apply IHM1.
+    assert (HF : (fun res1 : tm => CPS k F M2 (fun res2 : tm => continuation <{ res1 * res2 }>) (S (S n0)) fuel) = (fun res1 : tm => CPS k F M2 (fun res2 : tm => continuation <{ res1 * res2 }>) (S (n + S n0)) fuel)). {
+    apply stlc_functional_extensionality. intros. eapply S_Trans. apply S_Symm. apply IHM2. apply IHM2. } rewrite HF. apply IHM1.
+  - destruct fuel. simpl. apply S_Refl. simpl. destruct (find_func F M1), (find_func F M2). apply S_If0. apply S_Refl. apply IHM2. apply IHM3. apply S_If0. apply S_Refl. apply IHM2. apply IHM3.
+    apply IHM1. apply IHM1.
+  - destruct fuel. simpl. apply S_Refl. simpl. destruct (find_func F (continuation <{ nil }>)). apply S_Refl. apply S_Refl.
+  - destruct fuel. simpl. apply S_Refl. simpl. destruct (find_func F M1), (find_func F M2). apply S_Refl. apply IHM2. apply IHM1.
+    assert (HF : (fun res1 : tm => CPS k F M2 (fun res2 : tm => continuation <{ res1 :: res2 }>) (S (S n0)) fuel) = (fun res1 : tm => CPS k F M2 (fun res2 : tm => continuation <{ res1 :: res2 }>) (S (n + S n0)) fuel)). {
+    apply stlc_functional_extensionality. intros. eapply S_Trans. apply S_Symm. apply IHM2. apply IHM2. } rewrite HF. apply IHM1.
+  - destruct fuel. simpl. apply S_Refl. simpl. destruct (find_func F M1), (find_func F M2). apply S_LCase. apply S_Refl. apply IHM2. apply IHM3. apply S_LCase. apply S_Refl. apply IHM2. apply IHM3.
+    apply IHM1. apply IHM1.
+  - destruct fuel. simpl. apply S_Refl. simpl. apply S_Let. apply IHM1. apply IHM2.
+  - destruct fuel. simpl. apply S_Refl. simpl. apply S_Fix. apply IHM.
+Admitted.
 
+Lemma eqbP : forall n m, Bool.reflect (n = m) (n =? m)%string.
+Proof.
+  intros n m. apply Bool.iff_reflect. rewrite eqb_eq. reflexivity.
+Qed.
+
+Lemma in_distributive_by_app :
+  forall (F : string) (l1 l2 : list string), List.In F (l1 ++ l2) <-> (List.In F l1 \/ List.In F l2).
+Proof.
+  intros. split.
+  - intros H. induction l1; simpl in *.
+    + right. apply H.
+    + destruct H. left. left. apply H. destruct (IHl1 H). left. right. apply H0. right. apply H0.
+  - intros [H1 | H2].
+    + induction l1; simpl in *. exfalso. apply H1. destruct H1. left. apply H. right. apply (IHl1 H).
+    + induction l2; simpl in *. exfalso. apply H2. apply List.in_or_app. right. simpl. apply H2.
+Qed.
+
+Theorem substution_invariance :
+  forall F M f, (List.In F (list_name M) -> False) -> (subst F f M =s M).
+Proof.
+  intros. induction M; simpl in *.
+  - rewrite eqb_sym. destruct (eqbP s F). exfalso. apply H.
+    left. apply e. apply S_Refl.
+  - rewrite in_distributive_by_app in H. apply Decidable.not_or_iff in H. destruct H as [H1 H2].
+    apply S_App. apply IHM1. apply H1. apply IHM2. apply H2.
+  - rewrite eqb_sym. destruct (eqbP s F). apply S_Refl. apply S_Abs. apply Decidable.not_or_iff in H.
+    destruct H as [H1 H2]. apply (IHM H2).
+  - apply S_Refl.
+  - rewrite in_distributive_by_app in H. apply Decidable.not_or_iff in H. destruct H as [H1 H2].
+    apply S_Plus. apply IHM1. apply H1. apply IHM2. apply H2.
+  - rewrite in_distributive_by_app in H. apply Decidable.not_or_iff in H. destruct H as [H1 H2].
+    apply S_Minus. apply IHM1. apply H1. apply IHM2. apply H2.
+  - rewrite in_distributive_by_app in H. apply Decidable.not_or_iff in H. destruct H as [H1 H2].
+    apply S_Mult. apply IHM1. apply H1. apply IHM2. apply H2.
+  - rewrite in_distributive_by_app in H. rewrite in_distributive_by_app in H. apply Decidable.not_or_iff in H.
+    destruct H as [H1 H23]. apply Decidable.not_or_iff in H23. destruct H23 as [H2 H3]. apply S_If0. apply (IHM1 H1).
+    apply (IHM2 H2). apply (IHM3 H3).
+  - apply S_Refl.
+  - rewrite in_distributive_by_app in H. apply Decidable.not_or_iff in H. destruct H as [H1 H2].
+    apply S_Cons. apply IHM1. apply H1. apply IHM2. apply H2.
+  - rewrite in_distributive_by_app in H. rewrite in_distributive_by_app in H. apply Decidable.not_or_iff in H.
+    destruct H as [H1 H23]. apply Decidable.not_or_iff in H23. destruct H23 as [H2 H3]. apply S_LCase. apply (IHM1 H1).
+    apply (IHM2 H2). simpl in H3. rewrite eqb_sym. destruct (eqbP s F). apply S_Refl. rewrite eqb_sym. destruct (eqbP s0 F). apply S_Refl.
+    apply IHM3. apply Decidable.not_or_iff in H3. destruct H3. apply Decidable.not_or_iff in H0. destruct H0. apply H3.
+  - rewrite eqb_sym. rewrite in_distributive_by_app in H. apply Decidable.not_or_iff in H. destruct H as [H H12].
+    apply Decidable.not_or_iff in H12. destruct H12 as [H1 H2]. destruct (eqbP s F). apply S_Let. apply (IHM1 H1). apply S_Refl.
+    apply S_Let. apply (IHM1 H1). apply (IHM2 H2).
+  - apply S_Fix. apply IHM. apply H.
+Qed.
+
+Lemma str_reflect : forall s1 s2, s1 <> s2 -> (eqb s1 s2)%string = false.
+Proof.
+  intros. destruct (eqbP s1 s2). apply H in e. destruct e. reflexivity.
+Qed.
+
+Theorem subst_distribution :
+  forall F G f t1 t2, F <> G -> no_duplicate F t1 -> no_duplicate F t2 -> no_duplicate G t2 ->
+  subst F f (subst G t1 t2) =s subst G (subst F f t1) (subst F f t2).
+Proof.
+  intros F G f t1 t2. induction t2; intros HNeq HF1 HF2 HG2.
+  - simpl. destruct (eqbP F s), (eqbP G s). rewrite e in HNeq. rewrite e0 in HNeq. exfalso. apply HNeq. reflexivity.
+    simpl. rewrite e. rewrite eqb_refl. admit. simpl. rewrite e. rewrite eqb_refl. apply S_Refl. simpl.
+    rewrite (str_reflect F s n). rewrite (str_reflect G s n0). apply S_Refl. 
+  - simpl. apply S_App. apply IHt2_1. apply HNeq. apply HF1. inversion HF2. apply H1. inversion HG2. apply H1.
+    apply IHt2_2. apply HNeq. apply HF1. inversion HF2. apply H2. inversion HG2. apply H2.
+  - simpl. inversion HF2. inversion HG2. rewrite (str_reflect F s H1). rewrite (str_reflect G s H5). simpl.
+    rewrite (str_reflect F s H1). rewrite (str_reflect G s H5). apply S_Abs. apply IHt2. assumption. assumption.
+    assumption. assumption.
+  - simpl. apply S_Refl.
+  - simpl. apply S_Plus. apply IHt2_1. apply HNeq. apply HF1. inversion HF2. apply H1. inversion HG2. apply H1.
+    apply IHt2_2. apply HNeq. apply HF1. inversion HF2. apply H2. inversion HG2. apply H2.
+  - simpl. apply S_Minus. apply IHt2_1. apply HNeq. apply HF1. inversion HF2. apply H1. inversion HG2. apply H1.
+    apply IHt2_2. apply HNeq. apply HF1. inversion HF2. apply H2. inversion HG2. apply H2.
+  - simpl. apply S_Mult. apply IHt2_1. apply HNeq. apply HF1. inversion HF2. apply H1. inversion HG2. apply H1.
+    apply IHt2_2. apply HNeq. apply HF1. inversion HF2. apply H2. inversion HG2. apply H2.
+  - simpl. apply S_If0. apply IHt2_1. apply HNeq. apply HF1. inversion HF2. apply H2. inversion HG2. apply H2.
+    apply IHt2_2. apply HNeq. apply HF1. inversion HF2. apply H3. inversion HG2. apply H3. apply IHt2_3.
+    apply HNeq. apply HF1. inversion HF2. apply H4. inversion HG2. apply H4.
+  - simpl. apply S_Refl.
+  - simpl. apply S_Cons. apply IHt2_1. apply HNeq. apply HF1. inversion HF2. apply H1. inversion HG2. apply H1.
+    apply IHt2_2. apply HNeq. apply HF1. inversion HF2. apply H2. inversion HG2. apply H2.
+  - simpl. inversion HF2. inversion HG2. rewrite (str_reflect F s H4). rewrite (str_reflect G s H14). rewrite (str_reflect F s0 H5). rewrite (str_reflect G s0 H15).
+    apply S_LCase. apply IHt2_1. assumption. assumption. assumption. assumption. apply IHt2_2. assumption. assumption. assumption.
+    assumption. apply IHt2_3. assumption. assumption. assumption. assumption.
+  - simpl. inversion HF2. inversion HG2. rewrite (str_reflect F s H2). rewrite (str_reflect G s H8). apply S_Let. apply IHt2_1.
+    assumption. assumption. assumption. assumption. apply IHt2_2. assumption. assumption. assumption. assumption.
+  - simpl. apply S_Fix. apply IHt2. assumption. assumption. inversion HF2. assumption. inversion HG2. assumption.
+Admitted.
 (*
   The definition of [stlc_eqb] :
 
                     -----------------------------                       (S_Refl)
-                               x1 =s x1
+                              x1 =s x1
 
-                               x1 =s x2
+                              x1 =s x2
                     -----------------------------                       (S_Symm)
-                               x2 =s x1
+                              x2 =s x1
 
-                               x1 =s x2
-                               x2 =s x3
+                              x1 =s x2
+                              x2 =s x3
                     -----------------------------                       (S_Trans)
-                               x1 =s x3
+                              x1 =s x3
 
                               t1 =s t1'
                               t2 =s t2'
@@ -254,7 +420,7 @@ Proof.
 
                         In y (list_name t) = false
                     --------------------------------                    (S_AbsName)
-                          abs x t =s abs x t'
+                     abs x t =s abs y (subst x y t)
 
                               t1 =s t1'
                               t2 =s t2'
@@ -292,13 +458,21 @@ Proof.
                               t2 =s t2'
                               t3 =s t3'
                     ---------------------------------                   (S_LCase)
-                      tlcase t1 t2 x1 x2 t3 =s tlcase t1' t2' x1 x2 t3'
+              tlcase t1 t2 x1 x2 t3 =s tlcase t1' t2' x1 x2 t3'
 
             -----------------------------------------------------       (S_LCaseAppLeft)
       app k (tlcase t1 t2 x1 x2 t3) =s tlcase t1 (app k t2) x1 x2 (app k t3)
 
             -----------------------------------------------------       (S_LCaseAppRight)
       app (tlcase t1 t2 x1 x2 t3) k =s tlcase t1 (app t2 k) x1 x2 (app t3 k)
+
+                              t1 =s t1'
+                              t2 =s t2'
+                    ---------------------------------                   (S_Let)
+                     tlet x t1 t2 =s tlet x t1' t2'
+
+                    ---------------------------------                   (S_LetSubst)
+                     tlet x t1 t2 =s subst x t1 t2
 
                               t1 =s t1'
                     ---------------------------------                   (S_Fix)
@@ -329,6 +503,7 @@ Proof.
     Consequently we can get two lemmas:
     1. subst F f k =s k
     2. subst F f' k =s k
+    ▲ If k contains recursive call (as a intermediate state of the process), the conversion function will not apply it with [k].
 
   Our conversion function:
     CPS (k : tm) (func_name : string) (func_body : tm) (continuation : tm -> tm) (naming fuel : nat),
@@ -338,6 +513,9 @@ Proof.
     subst F f' (CPS k F M (fun res => res) 1 (depth F M)) =s app k (subst F f M)
 
   Proof:
+
+  First, if we say a stlc term [t] is recursive, we mean that [find_func F t > 0].
+  Here we note [find_func F t1 = S n1] and [find_func F t2 = S n2] if [t1] or [t2] is recursive.
 
   By induction on M.
 
@@ -356,8 +534,8 @@ Proof.
        =s app k (var x1)
        =s app k (subst F f (var x1))
 
-  2. When M = app t1 t2.
-  
+  2. When M = app t1 t2. (TODO)
+
   3. When M = tconst n.
      We know that,
           CPS k F (tconst n) (fun res => res) 1 (depth F (tconst n))
@@ -372,9 +550,9 @@ Proof.
 
   4. When M = tplus t1 t2.
      The induction hypothesis:
-          subst F f' (CPS k F t1 (fun res => res) 1 (depth F t1)) =s app k (subst F f t1)
-          subst F f' (CPS k F t2 (fun res => res) 1 (depth F t2)) =s app k (subst F f t2)
-       ▲ If both t1 and t2 are not resursive,
+            forall k, subst F f' (CPS k F t1 (fun res => res) 1 (depth F t1)) =s app k (subst F f t1)
+            forall k, subst F f' (CPS k F t2 (fun res => res) 1 (depth F t2)) =s app k (subst F f t2)
+     ▲ If both t1 and t2 are not resursive,
        We know that,
             CPS k F (tplus t1 t2) (fun res => res) 1 (depth F (tplus t1 t2))
          =s CPS k F (tplus t1 t2) (fun res => res) 1 1
@@ -386,45 +564,211 @@ Proof.
          =s app k (tplus t1 t2)
          =s app k (tplus (subst F f t1) (subst F f t2))
          =s app k (subst F f (tplus t1 t2))
-       ▲ If t1 is recursive and t2 not recursive,
+     ▲ If t1 is recursive and t2 not recursive,
        We know that,
             CPS k F (tplus t1 t2) (fun res => res) 1 (depth F (tplus t1 t2))
          =s CPS k F (tplus t1 t2) (fun res => res) 1 (1 + depth F t1)
-         =s CPS k F t1 (fun res : tm => tplus res t2) 1 (depth F t1)
-         =s (?)
+         =s CPS k F t1 (fun res => tplus res t2) 1 (depth F t1)
+       According to the induction hypothesis,
+            forall k, subst F f' (CPS k F t1 (fun res => res) 1 (depth F t1)) =s app k (subst F f t1)
+       We have,
+            subst F f' (CPS k F t1 (fun res => tplus res t2) 1 (depth F t1)) =s app k (tplus (subst F f t1) t2)
        Finally,
             subst F f' (CPS k F (tplus t1 t2) (fun res => res) 1 (depth F (tplus t1 t2)))
-         =s subst F f' (CPS k F t1 (fun res : tm => tplus res t2) 1 (depth F t1))
-         =s 
+         =s subst F f' (CPS k F t1 (fun res => tplus res t2) 1 (depth F t1))
          =s app k (tplus (subst F f t1) t2)
          =s app k (subst F f (tplus t1 t2))
-         
-         
-         
-         
+
+     ▲ If t2 is recursive and t1 not recursive,
+       We know that,
+            CPS k F (tplus t1 t2) (fun res => res) 1 (depth F (tplus t1 t2))
+         =s CPS k F (tplus t1 t2) (fun res => res) 1 (1 + depth F t2)
+         =s CPS k F t2 (fun res => tplus t1 res) 1 (depth F t2)
+       According to the induction hypothesis,
+            forall k, subst F f' (CPS k F t2 (fun res => res) 1 (depth F t2)) =s app k (subst F f t2)
+       We have,
+            subst F f' (CPS k F t2 (fun res => tplus t1 res) 1 (depth F t2)) =s app k (tplus t1 (subst F f t2))
+       Finally,
+            subst F f' (CPS k F (tplus t1 t2) (fun res => res) 1 (depth F (tplus t1 t2)))
+         =s subst F f' CPS k F t2 (fun res => tplus t1 res) 1 (depth F t2)
+         =s app k (tplus t1 (subst F f t2))
+         =s app k (subst F f (tplus t1 t2))
+
+     ▲ If both t1 and t2 are recursive,
+       We know that,
+            CPS k F (tplus t1 t2) (fun res => res) 1 (depth F (tplus t1 t2))
+         =s CPS k F (tplus t1 t2) (fun res => res) 1 (1 + max (depth F t1) (depth F t2))
+         =s CPS k F t1 (fun res1 => CPS k F t2 (fun res2 => tplus res1 res2)
+            (1 + (S n1)) (max (depth F t1) (depth F t2))) 1 (max (depth F t1) (depth F t2))
+       According to the induction hypothesis,
+            forall k, subst F f' (CPS k F t1 (fun res => res) 1 (depth F t1)) =s app k (subst F f t1)
+            forall k, subst F f' (CPS k F t2 (fun res => res) (1 + (S n1)) (depth F t2))
+         =s subst F f' (CPS k F t2 (fun res => res) 1 (depth F t2)) =s app k (subst F f t2)
+       We have,
+            subst F f' (CPS k F t1 (fun res1 => CPS k F t2 (fun res2 => tplus res1 res2)
+            (1 + (S n1)) (max (depth F t1) (depth F t2))) 1 (max (depth F t1) (depth F t2)))
+         =s subst F f' (CPS k F t1 (fun res1 => CPS k F t2 (fun res2 => tplus res1 res2)
+            (1 + (S n1)) (max (depth F t1) (depth F t2))) 1 (depth F t1))
+         =s subst F f' (CPS k F t2 (fun res2 => tplus t1 res2) (1 + (S n1)) (max (depth F t1) (depth F t2)))
+         =s subst F f' (CPS k F t2 (fun res2 => tplus t1 res2) (1 + (S n1)) (depth F t2))
+         =s app k (tplus (subst F f t1) (subst F f t2))
+      Finally,
+            subst F f' (CPS k F (tplus t1 t2) (fun res => res) 1 (depth F (tplus t1 t2)))
+         =s app k (tplus (subst F f t1) (subst F f t2))
+         =s app k (subst F f (tplus t1 t2))
+
+  Cases where M = tminus t1 t2, tmult t1 t2 and tcons t1 t2 are similar.
+
+  5. When M = tif0 t1 t2 t3.
+     The induction hypothesis:
+          forall k, subst F f' (CPS k F t1 (fun res => res) 1 (depth F t1)) =s app k (subst F f t1)
+          forall k, subst F f' (CPS k F t2 (fun res => res) 1 (depth F t2)) =s app k (subst F f t2)
+          forall k, subst F f' (CPS k F t3 (fun res => res) 1 (depth F t3)) =s app k (subst F f t3)
+     ▲ If t1 is not recursive,
+       We know that,
+            CPS k F (tif0 t1 t2 t3) (fun res => res) 1 (depth F (tif0 t1 t2 t3))
+         =s CPS k F (tif0 t1 t2 t3) (fun res => res) 1 (1 + max (depth F t2) (depth F t3))
+         =s tif0 t1 (CPS k F t2 (fun res => res) 1 (max (depth F t2) (depth F t3)))
+            (CPS k F t3 (fun res => res) 1 (max (depth F t2) (depth F t3)))
+         =s tif0 t1 (CPS k F t2 (fun res => res) 1 (depth F t2))
+            (CPS k F t3 (fun res => res) 1 (depth F t3))
+       Finally,
+            subst F f' (CPS k F (tif0 t1 t2 t3) (fun res => res) 1 (depth F (tif0 t1 t2 t3)))
+         =s subst F f' (tif0 t1 (CPS k F t2 (fun res => res) 1 (depth F t2))
+            (CPS k F t3 (fun res => res) 1 (depth F t3)))
+         =s tif0 (subst F f' t1) (subst F f' (CPS k F t2 (fun res => res) 1 (depth F t2)))
+            (subst F f' (CPS k F t3 (fun res => res) 1 (depth F t3)))
+         =s tif0 t1 (app k (subst F f t2)) (app k (subst F f t3))
+         =s app k (tif0 t1 (subst F f t2) (subst F f t3))
+         =s app k (tif0 (subst F f t1) (subst F f t2) (subst F f t3))
+         =s app k (subst F f (tif0 t1 t2 t3))
+       
+     ▲ If t1 is recursive,
+       We know that,
+            CPS k F (tif0 t1 t2 t3) (fun res => res) 1 (depth F (tif0 t1 t2 t3))
+         =s CPS k F (tif0 t1 t2 t3) (fun res => res) 1 (1 + max (depth F t1) (max (depth F t2) (depth F t3)))
+         =s CPS k F t1 (fun res => tif0 res
+            (CPS k F t2 (fun res => res) (1 + (S n1)) (max (depth F t1) (max (depth F t2) (depth F t3))))
+            (CPS k F t3 (fun res => res) (1 + (S n1)) (max (depth F t1) (max (depth F t2) (depth F t3))))) 1 (max (depth F t1) (max (depth F t2) (depth F t3)))
+       According to the induction hypothesis,
+            forall k, subst F f' (CPS k F t1 (fun res => res) 1 (depth F t1)) =s app k (subst F f t1)
+            forall k, subst F f' (CPS k F t2 (fun res => res) 1 (depth F t2)) =s app k (subst F f t2)
+            forall k, subst F f' (CPS k F t3 (fun res => res) 1 (depth F t3)) =s app k (subst F f t3)
+       We have,
+            subst F f' (CPS k F t2 (fun res => res) (1 + (S n1)) (max (depth F t1) (max (depth F t2) (depth F t3))))
+         =s subst F f' (CPS k F t2 (fun res => res) (1 + (S n1)) (depth F t2))
+         =s subst F f' (CPS k F t2 (fun res => res) 1 (depth F t2))
+         =s app k (subst F f t2)
+            subst F f' (CPS k F t3 (fun res => res) (1 + (S n1)) (max (depth F t1) (max (depth F t2) (depth F t3))))
+         =s subst F f' (CPS k F t3 (fun res => res) (1 + (S n1)) (depth F t3))
+         =s subst F f' (CPS k F t3 (fun res => res) 1 (depth F t3))
+         =s app k (subst F f t3)
+            subst F f' (CPS k F t1 (fun res => tif0 res
+            (CPS k F t2 (fun res => res) (1 + (S n1)) (max (depth F t1) (max (depth F t2) (depth F t3))))
+            (CPS k F t3 (fun res => res) (1 + (S n1)) (max (depth F t1) (max (depth F t2) (depth F t3))))) 1 (max (depth F t1) (max (depth F t2) (depth F t3))))
+         =s subst F f' (CPS k F t1 (fun res => tif0 res
+            (CPS k F t2 (fun res => res) (1 + (S n1)) (max (depth F t1) (max (depth F t2) (depth F t3))))
+            (CPS k F t3 (fun res => res) (1 + (S n1)) (max (depth F t1) (max (depth F t2) (depth F t3))))) 1 (depth F t1))
+         =s tif0 (subst F f t1) (subst F f' (CPS k F t2 (fun res => res) (1 + (S n1)) (max (depth F t1) (max (depth F t2) (depth F t3)))))
+            (subst F f' (CPS k F t3 (fun res => res) (1 + (S n1)) (max (depth F t1) (max (depth F t2) (depth F t3)))))
+         =s tif0 (subst F f t1) (subst F f' (CPS k F t2 (fun res => res) (1 + (S n1)) (depth F t2)))
+            (subst F f' (CPS k F t3 (fun res => res) (1 + (S n1)) (depth F t3)))
+         =s tif0 (subst F f t1) (app k (subst F f t2)) (app k (subst F f t3))
+        
+       Finally,
+            subst F f' (CPS k F (tif0 t1 t2 t3) (fun res => res) 1 (depth F (tif0 t1 t2 t3)))
+         =s tif0 (subst F f t1) (app k (subst F f t2)) (app k (subst F f t3))
+         =s app k (tif0 (subst F f t1) (subst F f t2) (subst F f t3))
+         =s app k (subst F f (tif0 t1 t2 t3))
+
+  The case where M = tlcase t1 t2 x1 x2 t3 is similar.
+
+  6. When M = tnil.
+     We know that,
+          CPS k F tnil (fun res => res) 1 (depth F tnil)
+       =s CPS k F nil (fun res => res) 1 1
+       =s app k nil
+     Finally,
+          subst F f' (CPS k F tnil (fun res => res) 1 (depth F tnil))
+       =s subst F f' (app k nil)
+       =s app k nil
+       =s app k (subst F f nil)
+   
+  7. When M = tlet x1 t1 t2.
+     The induction hypothesis:
+            forall k, subst F f' (CPS k F t1 (fun res => res) 1 (depth F t1)) =s app k (subst F f t1)
+            forall k, subst F f' (CPS k F t2 (fun res => res) 1 (depth F t2)) =s app k (subst F f t2)
+     ▲ If both t1 and t2 are not resursive,
+       We know that,
+            CPS k F (tlet x1 t1 t2) (fun res => res) 1 (depth F (tlet x1 t1 t2))
+         =s CPS k F (tlet x1 t1 t2) (fun res => res) 1 1
+         =s app k (tlet x1 t1 t2)
+       Finally,
+            subst F f' (CPS k F (tlet x1 t1 t2) (fun res => res) 1 (depth F (tlet x1 t1 t2)))
+         =s subst F f' (app k (tlet x1 t1 t2))
+         =s app (subst F f' k) (tlet x1 (subst F f' t1) (subst F f' t2))
+         =s app k (tlet x1 t1 t2)
+         =s app k (tlet x1 (subst F f t1) (subst F f t2))
+         =s app k (subst F f (tlet x1 t1 t2))
+     ▲ If t1 is recursive and t2 not recursive,
+       We know that,
+            CPS k F (tlet x1 t1 t2) (fun res => res) 1 (depth F (tlet x1 t1 t2))
+         =s CPS k F (tlet x1 t1 t2) (fun res => res) 1 (1 + depth F t1)
+         =s CPS (abs res res) F t1 (fun res : tm => tlet x1 res (app k t2)) 1 (depth F t1)
+       According to the induction hypothesis,
+            forall k, subst F f' (CPS k F t1 (fun res => res) 1 (depth F t1)) =s app k (subst F f t1)
+       We have,
+            subst F f' (CPS (abs res res) F t1 (fun res : tm => tlet x1 res (app k t2)) 1 (depth F t1))
+         =s app k (tlet x1 (subst F f t1) (app k t2))
+       Finally,
+            subst F f' (CPS k F (tlet x1 t1 t2) (fun res => res) 1 (depth F (tlet x1 t1 t2)))
+         =s app (abs res res) (tlet x1 (subst F f t1) (app k t2))
+         =s tlet x1 (subst F f t1) (app k t2)
+         =s subst x1 (subst F f t1) (app k t2)
+         =s app (subst x1 (subst F f t1) k) (subst x1 (subst F f t1) t2)
+         =s app k (subst x1 (subst F f t1) t2)
+         =s app k (subst x1 (subst F f t1) (subst F f t2))
+         =s app k (subst F f (subst x1 t1 t2))
+         =s app k (subst F f (tlet x1 t1 t2))
+
+     ▲ If t2 is recursive and t1 not recursive,
+       We know that,
+            CPS k F (tlet x1 t1 t2) (fun res => res) 1 (depth F (tlet x1 t1 t2))
+         =s CPS k F (tlet x1 t1 t2) (fun res => res) 1 (1 + depth F t2)
+         =s CPS k F t2 (fun res : tm => tlet x1 t1 res) 1 (depth F t2)
+       According to the induction hypothesis,
+            forall k, subst F f' (CPS k F t2 (fun res => res) 1 (depth F t2)) =s app k (subst F f t2)
+       We have,
+            subst F f' (CPS k F t2 (fun res : tm => tlet x1 t1 res) 1 (depth F t2))
+         =s app k (tlet x1 t1 (subst F f t2))
+       Finally,
+            subst F f' (CPS k F (tlet x1 t1 t2) (fun res => res) 1 (depth F (tlet x1 t1 t2)))
+         =s app k (tlet x1 t1 (subst F f t2))
+         =s app k (tlet x1 (subst F f t1) (subst F f t2))
+         =s app k (subst F f (tlet x1 t1 t2))
+
+     ▲ If both t1 and t2 are recursive,
+       We know that,
+            CPS k F (tlet x1 t1 t2) (fun res => res) 1 (depth F (tlet x1 t1 t2))
+         =s CPS k F (tlet x1 t1 t2) (fun res => res) 1 (1 + max (depth F t1) (depth F t2))
+         =s CPS (abs res res) F t1 (fun res1 => CPS k F t2 (fun res2 => tlet x1 res1 res2)
+            (1 + (S n1)) (max (depth F t1) (depth F t2))) 1 (max (depth F t1) (depth F t2))
+       According to the induction hypothesis,
+            forall k, subst F f' (CPS k F t1 (fun res => res) 1 (depth F t1)) =s app k (subst F f t1)
+            forall k, subst F f' (CPS k F t2 (fun res => res) (1 + (S n1)) (depth F t2))
+            =s subst F f' (CPS k F t2 (fun res => res) 1 (depth F t2)) =s app k (subst F f t2)
+       We have,
+            subst F f' (CPS (abs res res) F t1 (fun res1 => CPS k F t2 (fun res2 => tlet x1 res1 res2)
+            (1 + (S n1)) (max (depth F t1) (depth F t2))) 1 (max (depth F t1) (depth F t2)))
+         =s subst F f' (CPS (abs res res) F t1 (fun res1 => CPS k F t2 (fun res2 => tlet x1 res1 res2)
+            (1 + (S n1)) (max (depth F t1) (depth F t2))) 1 (depth F t1))
+         =s subst F f' (CPS k F t2 (fun res2 => tlet x1 t1 res2) (1 + (S n1)) (max (depth F t1) (depth F t2)))
+         =s subst F f' (CPS k F t2 (fun res2 => tlet x1 t1 res2) (1 + (S n1)) (depth F t2))
+         =s app k (tlet x1 (subst F f t1) (subst F f t2))
+       Finally,
+            CPS k F (tlet x1 t1 t2) (fun res => res) 1 (depth F (tlet x1 t1 t2))
+         =s app k (tlet x1 (subst F f t1) (subst F f t2))
+         =s app k (subst x1 (subst F f t1) (subst F f t2))
+         =s app k (subst F f (subst x1 t1 t2))
+         =s app k (subst F f (tlet x1 t1 t2))
 *)
-
-Compute 1.
-
-Compute (CPS k F 
-<{ F a (F b c) }>
- (fun res => res) 1 (depth F <{ F a (F b c) }>)).
-
-Compute (CPS k F 
-<{ F a (F b c) }>
- (fun res => tplus res n2) 1 (depth F <{ F a (F b c) }>)).
-
-Compute (CPS k F 
-<{ F a (F b c) + n2 }>
- (fun res => res) 1 (depth F <{ F a (F b c) + n2 }>)).
-
-Compute (tplus (CPS k F <{ F a (F b c) }> (fun res => res) 1 (depth F <{ F a (F b c) }>)) n2).
-
-Compute (CPS k F 
-<{ F a (F b c) }>
- (fun res => res) 1 (depth F <{ F a (F b c) }>)).
-
-
-
-
-
