STLC/Examples.v
@@ -1,0 +1,46 @@
+From STLC Require Export Argument.
+
+(*
+  F l1 :=
+    match l1 with
+    | nil => 2
+    | n1 :: l1' => 1 + match l1' with
+                       | nil => 2
+                       | n2 :: l2' => n1 + n2 + F l2'
+                       end
+    end.
+  We can transfer it to CPS-style by hand:
+  F l1 k :=
+    match l1 with
+    | nil => k 2
+    | n1 :: l1' => match l1' with
+                   | nil => k (1 + 2)
+                   | n2 :: l2' => F l2' (fun res1 => k (1 + (n1 + n2 + res1)))
+                   end
+    end.
+*)
+
+Definition stlc_example_1 :=
+  tfix (abs F (abs l1
+    (tlcase l1 2 n1 l1'
+      (tplus 1 (tlcase l1' 2 n2 l2'
+        (tplus (tplus n1 n2) (app F l2'))))))).
+
+Compute (CPS_conversion stlc_example_1).
+
+(*
+  F n1 n2 n3 :=
+    1 + match F n1 n2 n3 with
+        | 0 => 2 + F n1 n2 (n3 - 1)
+        | S _ => 3 + F n1 n2 (n3 - 2)
+        end
+*)
+
+Definition stlc_example_2 :=
+  tfix (abs F (abs n1 (abs n2 (abs n'
+    (tplus 1 (tif0 (app (app (app F n1) n2) n')
+      (tplus 2 (app (app (app F n1) n2) (tminus n' 1)))
+        (tplus 3 (app (app (app F n1) n2) (tminus n' 2))))))))).
+        
+Compute (CPS_conversion stlc_example_2).
+        
